expr adequacy and partial cmd adequacy (missing Call)

theories/semtype_alt.v
@@ -6,44 +6,6 @@ From iris.proofmode Require Import tactics.
 
 Definition tag := string.
 
-Inductive ty :=
-  | IntT
-  | BoolT
-  | NothingT
-  | MixedT
-  | ClassT (cname: tag)
-  | NullT
-  | NonNullT
-  | UnionT (s t: ty)
-  | InterT (s t: ty)
-.
-
-Record methodDef := {
-  methodname: string;
-  methodargs: list (string * ty)%type;
-  methodrettype: ty;
-  (* methodbody: comm; *)
-}.
-
-Record classDef := {
-  classname: tag;
-  superclass: option tag;
-  classfields : stringmap ty;
-  classmethods : stringmap methodDef;
-}.
-
-Definition loc := positive.
-
-Global Instance loc_dec_eq (l l' : loc) : Decision (l = l') := _.
-
-Inductive value : Set :=
-  | IntV (z: Z)
-  | BoolV (b: bool)
-  | NullV
-  | LocV (ℓ : loc).
-
-Local Instance value_inhabited : Inhabited value := populate NullV.
-
 Local Instance tag_equiv : Equiv tag := fun s0 s1 => String.eqb s0 s1 = true.
 Local Instance tag_equivalence : Equivalence (≡@{tag}).
 Proof.
@@ -58,136 +20,83 @@ Qed.
 
 Canonical Structure tagO : ofe := leibnizO tag.
 
-(* interpretation of ty *)
+Definition loc := positive.
+Global Instance loc_dec_eq (l l' : loc) : Decision (l = l') := _.
+
+Inductive value : Set :=
+  | IntV (z: Z)
+  | BoolV (b: bool)
+  | NullV
+  | LocV (ℓ : loc).
+Local Instance value_inhabited : Inhabited value := populate NullV.
+
+(* interpretation of types *)
 Definition sem_typeO (Σ : gFunctors) : ofe := value -d> iPropO Σ.
 
 Class sem_heapG (Σ : gFunctors) : Set := SemHeapG {
   sem_heapG_heap :> inG Σ (gmap_viewR loc (prodO tagO (gmapO string (laterO (sem_typeO Σ)))));
 }.
 
+Inductive lang_ty :=
+  | IntT
+  | BoolT
+  | NothingT
+  | MixedT
+  | ClassT (cname: tag)
+  | NullT
+  | NonNullT
+  | UnionT (s t: lang_ty)
+  | InterT (s t: lang_ty)
+.
+Canonical Structure lang_tyO : ofe := leibnizO lang_ty.
+
+Definition var := string.
+Global Instance var_dec_eq (l l' : var) : Decision (l = l') := _.
+
+Inductive primop :=
+  | PlusO | MinusO | TimesO | DivO | LeqO | GeqO | EqO
+.
+
+Inductive expr :=
+  | IntE (z: Z)
+  | BoolE (b: bool)
+  | NullE
+  | OpE (op: primop) (e1: expr) (e2: expr)
+  | VarE (v: var)
+.
+
+Inductive cmd : Set :=
+  | SkipC
+  | SeqC (fstc: cmd) (sndc: cmd)
+  | LetC (lhs: var) (e: expr)
+  | IfC (cond: expr) (thn: cmd) (els: cmd)
+  | CallC (lhs: var) (recv: expr) (name: string) (args: stringmap expr)
+  | NewC (lhs: var) (class_name: tag) (args: stringmap expr)
+  | GetC (lhs: var) (recv: expr) (name: string)
+  | SetC (recv: expr) (fld: string) (rhs: expr)
+.
+
+Record methodDef := {
+  methodname: string;
+  methodargs: stringmap lang_ty;
+  methodrettype: lang_ty;
+  methodbody: cmd;
+  methodret: expr;
+}.
+
+Record classDef := {
+  classname: tag;
+  superclass: option tag;
+  classfields : stringmap lang_ty;
+  classmethods : stringmap methodDef;
+}.
+
 Section proofs.
 Context `{!sem_heapG Σ}.
-Context (Δ: stringmap classDef).
 Notation iProp := (iProp Σ).
 
-Inductive ancestor (target: tag) : tag -> Prop :=
-  | ARefl : ancestor target target
-  | ASuper current super cdef :
-      Δ !! current = Some cdef ->
-      cdef.(superclass) = Some super ->
-      ancestor target super ->
-      ancestor target current
-.
-Hint Constructors ancestor : core.
-
-Local Notation "A '`inherits`' B" := (ancestor B A) (at level 70, no associativity).
-
-Lemma inherits_trans:
-  forall A B C,
-  A `inherits` B -> B `inherits` C -> A `inherits` C.
-Proof.
-  intros A B C h; revert C.
-  induction h as [ | current super cdef hin hsuper h hi]; intros C hC; first by done.
-  econstructor; [ exact hin | exact hsuper | ].
-  now apply hi.
-Qed.
-
-(* Note useful, just for sanity check: extends are chains.
- * if A extends B and C, then either B extends C or C extends B.
- *)
-Corollary inherits_is_chain:
-  forall A B C,
-   A `inherits` B -> A `inherits` C->
-  (C `inherits` B \/ B `inherits` C).
-Proof.
-  intros A B C h; revert C.
-  induction h as [ | current super cdef hin hsuper h hi]; intros C hCA; first by right.
-  destruct hCA as [ | current' super' cdef' hin' hsuper' h'].
-  - left; econstructor; [ exact hin | exact hsuper | exact h].
-  - rewrite hin in hin'; injection hin'; intro heq; subst; clear hin hin'.
-    rewrite hsuper in hsuper'; injection hsuper'; intro heq; subst; clear hsuper hsuper'.
-    destruct (hi C h') as [ hC | hC ]; first by left.
-    by right.
-Qed.
-
-(* has_field fname ty cname checks if the class cname has a field named fname of type ty *)
-Inductive has_field (fname: string) (typ: ty): tag -> Prop :=
-  | HasField current cdef:
-      Δ !! current = Some cdef ->
-      cdef.(classfields) !! fname = Some typ ->
-      has_field fname typ current
-  | InheritsField current parent cdef:
-      Δ !! current = Some cdef ->
-      cdef.(classfields) !! fname = None ->
-      cdef.(superclass) = Some parent ->
-      has_field fname typ parent ->
-      has_field fname typ current.
-
-Hint Constructors has_field : core.
-
-(* all fields of class cname are in the fnames set *)
-Definition has_fields (cname: tag) (fnames: stringmap ty) : Prop :=
-  ∀ fname typ, has_field fname typ cname ↔ fnames !! fname = Some typ.
-
-Lemma has_fields_fun: forall c fs0 fs1,
-  has_fields c fs0 -> has_fields c fs1 -> fs0 = fs1.
-Proof.
-move => c fs0 fs1 h0 h1.
-apply map_eq => k.
-destruct (fs0 !! k) as [ ty | ] eqn:hty.
-- destruct (h1 k ty) as [hl1 hr1].
-  rewrite hl1 //=.
-  by apply h0.
-- destruct (fs1 !! k) as [ ty | ] eqn:hty'; last done.
-  destruct (h1 k ty) as [hl1 hr1].
-  apply h0 in hr1; last done.
-  by rewrite hty in hr1.
-Qed.
-
-Inductive subtype : ty -> ty -> Prop :=
-  | SubMixed : forall ty, subtype ty MixedT
-  | SubClass : forall A B, A `inherits` B -> subtype (ClassT A) (ClassT B)
-  | SubMixed2: subtype MixedT (UnionT NonNullT NullT)
-  | SubIntNonNull: subtype IntT NonNullT
-  | SubBoolNonNull: subtype BoolT NonNullT
-  | SubClassNonNull: forall A, subtype (ClassT A) NonNullT
-  | SubUnionUpper1 : forall s t, subtype s (UnionT s t)
-  | SubUnionUpper2 : forall s t, subtype t (UnionT s t)
-  (* Do we need this one *)
-  | SubUnionLeast : forall s t u, subtype s u -> subtype t u -> subtype (UnionT s t) u
-  | SubInterLower1 : forall s t, subtype (InterT s t) s
-  | SubInterLower2 : forall s t, subtype (InterT s t) t
-  | SubInterGreatest: forall s t u, subtype u s -> subtype u t -> subtype u (InterT s t)
-  | SubRefl: forall s, subtype s s
-  | SubTrans : forall s t u, subtype s t -> subtype t u -> subtype s u
-.
-
-Hint Constructors subtype : core.
-
-Notation "s <: t" := (subtype s t) (at level 70, no associativity).
-
-(* Derived rules *)
-Lemma subtype_union_comm : forall A B, (UnionT A B) <: (UnionT B A).
-Proof.
-by auto.
-Qed.
-
-Lemma subtype_inter_comm : forall A B, (InterT A B) <: (InterT B A).
-Proof.
-by auto.
-Qed.
-
-Lemma subtype_union_assoc:
-  forall A B C, (UnionT (UnionT A B) C) <: (UnionT A (UnionT B C)).
-Proof.
-by eauto.
-Qed.
-
-Lemma subtype_inter_assoc:
-  forall A B C, (InterT (InterT A B) C) <: (InterT A (InterT B C)).
-Proof.
-by eauto.
-Qed.
+(* assume a given set of class definitions *)
+Context (Δ: stringmap classDef).
 
 (* the interpretation of types is simply given by
    the carrier set of the sem_typeO ofe *)
@@ -196,14 +105,6 @@ Definition interp := ofe_car interpO.
 Eval hnf in interp.
 (* = value → iPropO Σ *)
 (*      : Type *)
-
-(* name for the semantic heap *)
-Context (γ : gname).
-
-Notation sem_heap_mapsto ℓ t iFs :=
-  (own γ (gmap_view_frag ℓ DfracDiscarded (t, iFs))).
-
-Notation ty_interpO := (ty -d> interpO).
 
 (* now, let's interpret some ty *)
 
@@ -225,6 +126,15 @@ Definition interp_inter (iA : interp) (iB : interp) : interp :=
 Definition interp_nothing : interp :=
   λ (_: value), False%I.
 
+(* name for the semantic heap *)
+Context (γ : gname).
+
+Notation sem_heap_mapsto ℓ t iFs :=
+  (own γ (gmap_view_frag ℓ DfracDiscarded (t, iFs))).
+
+Notation ty_interpO := (lang_ty -d> interpO).
+
+
 Definition interp_nonnull : interp :=
   λ (v : value),
      ((∃ z, ⌜v = IntV z⌝) ∨
@@ -233,25 +143,133 @@ Definition interp_nonnull : interp :=
 
 Definition interp_mixed : interp :=
  λ (v: value), (interp_nonnull v ∨ interp_null v)%I.
-
 (* I need these two intermediate definition to make Coq/Type Classes instaces
  * happy.
  *)
-Definition interp_ty_next (rec: ty_interpO) (typ: ty): laterO interpO :=
+Definition interp_ty_next (rec: ty_interpO) (typ: lang_ty): laterO interpO :=
   Next (rec typ)
 .
 
-Definition interp_tys_next (rec: ty_interpO) (ftys: stringmap ty) : gmapO string (laterO interpO) :=
+Definition interp_tys_next (rec: ty_interpO) (ftys: stringmap lang_ty) : gmapO string (laterO interpO) :=
   (interp_ty_next rec) <$> ftys
 .
 
+(* class A extends B *)
+Definition extends (A B: tag) : Prop :=
+  exists cdef,
+  Δ !! A = Some cdef /\
+  cdef.(superclass) = Some B
+.
+
+(* Refl trans closure of extends *)
+Definition inherits := rtc extends.
+
+(* Note useful, just for sanity check: inherits are chains.
+ * if A inherits B and C, then either B inherits C or C inherits B.
+ *)
+Corollary inherits_is_chain:
+  forall A B C,
+   inherits A B -> inherits A C->
+  (inherits C B \/ inherits B C).
+Proof.
+  intros A B C h; revert C.
+  induction h as [ t | x y z hxy hyz hi]; move => c hc; first by right.
+   destruct hxy as (cdef & hin & hs).
+   destruct hc as [ t | u v w huv hvw].
+   - left; econstructor; first by exists cdef. done.
+   - destruct huv as (? & hin' & hs').
+     rewrite hin' in hin.
+     injection hin; intros ->; clear hin hin'.
+     rewrite hs' in hs.
+     injection hs; intros ->; clear hs hs'.
+     apply hi in hvw as [h | h]; first by left.
+     by right.
+Qed.
+
+(* has_field fname ty cname checks if the class cname has a field named fname of type ty *)
+Inductive has_field (fname: string) (typ: lang_ty): tag -> Prop :=
+  | HasField current cdef:
+      Δ !! current = Some cdef ->
+      cdef.(classfields) !! fname = Some typ ->
+      has_field fname typ current
+  | InheritsField current parent cdef:
+      Δ !! current = Some cdef ->
+      cdef.(classfields) !! fname = None ->
+      cdef.(superclass) = Some parent ->
+      has_field fname typ parent ->
+      has_field fname typ current.
+
+Hint Constructors has_field : core.
+
+(* A class cannot redeclare a field if it is present in
+ * any of its parent definition.
+ *)
+Definition wf_cdef_fields cdef : Prop :=
+  forall f fty super,
+  cdef.(superclass) = Some super ->
+  has_field f fty super ->
+  cdef.(classfields) !! f = None.
+
+Definition wf_cdefs (prog: stringmap classDef)  : Prop :=
+  map_Forall (fun cname cdef => wf_cdef_fields cdef) prog.
+
+(* all fields of class cname are in the fnames set *)
+Definition has_fields (cname: tag) (fnames: stringmap lang_ty) : Prop :=
+  ∀ fname typ, has_field fname typ cname ↔ fnames !! fname = Some typ.
+
+Lemma has_fields_fun: forall c fs0 fs1,
+  has_fields c fs0 -> has_fields c fs1 -> fs0 = fs1.
+Proof.
+move => c fs0 fs1 h0 h1.
+apply map_eq => k.
+destruct (fs0 !! k) as [ ty | ] eqn:hty.
+- destruct (h1 k ty) as [hl1 hr1].
+  rewrite hl1 //=.
+  by apply h0.
+- destruct (fs1 !! k) as [ ty | ] eqn:hty'; last done.
+  destruct (h1 k ty) as [hl1 hr1].
+  apply h0 in hr1; last done.
+  by rewrite hty in hr1.
+Qed.
+
+Ltac inv H := inversion H; subst; clear H.
+
+Lemma has_fields_inherits : wf_cdefs Δ -> forall A B, inherits A B ->
+  forall f fty, has_field f fty B -> has_field f fty A.
+Proof.
+move => wfΔ A B h.
+induction h as [ t | x y z hxy hyz hi]; move => f fty hf; first done.
+apply hi in hf.
+destruct hxy as (cdef & hΔ & hs).
+apply InheritsField with y cdef; move => //.
+apply wfΔ in hΔ.
+eapply hΔ; first done.
+done.
+Qed.
+
+Corollary has_fields_inherits_lookup:
+  wf_cdefs Δ ->
+  forall A B cdef name fty fields,
+  Δ !! B = Some cdef ->
+  classfields cdef !! name = Some fty ->
+  inherits A B ->
+  has_fields A fields ->
+  fields !! name = Some fty.
+Proof.
+  move => wfΔ A B cdef name fty fields hin hfields hinherits hf.
+  destruct (hf name fty) as [hl hr].
+  apply hl.
+  eapply (has_fields_inherits wfΔ); first done.
+  econstructor; first done.
+  done.
+Qed.
 
 (* interpret a class type given the tag and the
    interpretation of their fields *)
 Definition interp_class (cname : tag) (rec : ty_interpO) : interp :=
   λ (w : value),
-    (∃ ℓ t (fields:stringmap ty),
-    ⌜w = LocV ℓ ∧ t `inherits` cname ∧ has_fields t fields⌝ ∗
+    (∃ ℓ t (fields:stringmap lang_ty),
+    ⌜w = LocV ℓ ∧ inherits t cname ∧ has_fields t fields⌝ ∗
     sem_heap_mapsto ℓ t (interp_tys_next rec fields))%I.
 
 (* we use a blend of Coq/Iris recursion, the
@@ -259,8 +277,8 @@ Definition interp_class (cname : tag) (rec : ty_interpO) : interp :=
    cases, and we use Iris' recursion to deal with
    the more complicated case of class types *)
 Definition interp_type_pre (rec : ty_interpO) : ty_interpO :=
-  λ (typ : ty),
-    (fix go (typ : ty) : interp :=
+  λ (typ : lang_ty),
+    (fix go (typ : lang_ty) : interp :=
        match typ with
        | IntT => interp_int
        | BoolT => interp_bool
@@ -313,7 +331,7 @@ Qed.
    can be (mutually) recursive) *)
 Definition interp_type := fixpoint interp_type_pre.
 
-Lemma interp_type_unfold (ty : ty) (v : value) :
+Lemma interp_type_unfold (ty : lang_ty) (v : value) :
   interp_type ty v ⊣⊢ interp_type_pre interp_type ty v.
 Proof.
   rewrite {1}/interp_type.
@@ -329,6 +347,71 @@ elim => [ | | | | cname | | |s hs t ht | s hs t ht] v;
   by apply bi.or_persistent; rewrite -!interp_type_unfold.
 - rewrite /interp_union.
   by apply bi.and_persistent; rewrite -!interp_type_unfold.
+Qed.
+
+(*
+(* that is a bit of an awkward lemma;
+   I am not yet sure it "scales" *)
+Lemma interp_type_loc_inversion ty ℓ :
+  interp_type ty (LocV ℓ) -∗
+  ∃ t, interp_type (ClassT t) (LocV ℓ).
+Proof.
+  rewrite interp_type_unfold. elim: ty => /=.
+  - iIntros "%". naive_solver.
+  - move=>? IH1 ? IH2. iIntros "[H|H]".
+    by iApply IH1. by iApply IH2.
+  - move=> t. iIntros "H". iExists t.
+    by rewrite interp_type_unfold /=.
+Qed.
+ *)
+
+Lemma dom_interp_tys_next fields:
+  dom stringset (interp_tys_next interp_type fields) ≡ dom _ fields.
+Proof. by rewrite /interp_tys_next /interp_ty_next dom_fmap. Qed.
+
+Inductive subtype : lang_ty -> lang_ty -> Prop :=
+  | SubMixed : forall ty, subtype ty MixedT
+  | SubClass : forall A B, inherits A B -> subtype (ClassT A) (ClassT B)
+  | SubMixed2: subtype MixedT (UnionT NonNullT NullT)
+  | SubIntNonNull: subtype IntT NonNullT
+  | SubBoolNonNull: subtype BoolT NonNullT
+  | SubClassNonNull: forall A, subtype (ClassT A) NonNullT
+  | SubUnionUpper1 : forall s t, subtype s (UnionT s t)
+  | SubUnionUpper2 : forall s t, subtype t (UnionT s t)
+  (* Do we need this one *)
+  | SubUnionLeast : forall s t u, subtype s u -> subtype t u -> subtype (UnionT s t) u
+  | SubInterLower1 : forall s t, subtype (InterT s t) s
+  | SubInterLower2 : forall s t, subtype (InterT s t) t
+  | SubInterGreatest: forall s t u, subtype u s -> subtype u t -> subtype u (InterT s t)
+  | SubRefl: forall s, subtype s s
+  | SubTrans : forall s t u, subtype s t -> subtype t u -> subtype s u
+.
+
+Hint Constructors subtype : core.
+
+Notation "s <: t" := (subtype s t) (at level 70, no associativity).
+
+(* Derived rules *)
+Lemma subtype_union_comm : forall A B, (UnionT A B) <: (UnionT B A).
+Proof.
+by auto.
+Qed.
+
+Lemma subtype_inter_comm : forall A B, (InterT A B) <: (InterT B A).
+Proof.
+by auto.
+Qed.
+
+Lemma subtype_union_assoc:
+  forall A B C, (UnionT (UnionT A B) C) <: (UnionT A (UnionT B C)).
+Proof.
+by eauto.
+Qed.
+
+Lemma subtype_inter_assoc:
+  forall A B C, (InterT (InterT A B) C) <: (InterT A (InterT B C)).
+Proof.
+by eauto.
 Qed.
 
 
@@ -374,8 +457,8 @@ induction 1 as [A | A B hext | | | | A | A B| A B | A B C h0 hi0 h1 hi1
   iExists ℓ, t, fields.
   iSplit.
   { iPureIntro; split; first by done.
-    split ; first by eapply inherits_trans.
-    done.
+    split; last done.
+    by eapply rtc_transitive.
   }
   by iFrame.
 - by rewrite /= /interp_mixed.
@@ -412,11 +495,11 @@ induction 1 as [A | A B hext | | | | A | A B| A B | A B C h0 hi0 h1 hi1
   by iApply hi0.
 Qed.
 
-Lemma inherits_is_sub: forall C D, D `inherits` C -> (ClassT D) <: (ClassT C).
+Lemma inherits_is_sub: forall C D, inherits D C -> (ClassT D) <: (ClassT C).
 Proof.  by eauto. Qed.
 
 Lemma interp_type_inherits (l : loc) (C D: tag):
-  D `inherits` C ->
+  inherits D C ->
   interp_type (ClassT D) (LocV l) -∗
   interp_type (ClassT C) (LocV l).
 Proof.
@@ -425,360 +508,673 @@ iIntros "h".
 iApply subtype_is_inclusion; first by apply inherits_is_sub.
 done.
 Qed.
+(* language statics & semantics *)
+
+Definition local_tys := stringmap lang_ty.
+
+Inductive expr_has_ty (lty : local_tys) :
+    expr → lang_ty → Prop :=
+  | IntTy : forall z, expr_has_ty lty (IntE z) IntT
+  | BoolTy: forall b, expr_has_ty lty (BoolE b) BoolT
+  | NullTy: expr_has_ty lty NullE NullT
+  | OpIntTy: forall op e1 e2,
+      match op with
+      | PlusO | MinusO | TimesO | DivO => True
+          | _ => False
+      end → 
+      expr_has_ty lty e1 IntT →
+      expr_has_ty lty e2 IntT →
+      expr_has_ty lty (OpE op e1 e2) IntT
+  | OpBoolTy: forall op e1 e2,
+      match op with
+      | LeqO | GeqO | EqO => True
+      | _ => False
+      end → 
+      expr_has_ty lty e1 IntT →
+      expr_has_ty lty e2 IntT →
+      expr_has_ty lty (OpE op e1 e2) BoolT
+  | VarTy: forall v ty,
+      lty !! v = Some ty →
+      expr_has_ty lty (VarE v) ty
+.
+
+(* continuation-based typing for commands *)
+Inductive cmd_has_ty :
+    local_tys → cmd → local_tys → Prop :=
+  | SkipTy: forall lty, cmd_has_ty lty SkipC lty
+  | SeqTy: forall lty1 lty2 lty3 fstc sndc,
+      cmd_has_ty lty1 fstc lty2 →
+      cmd_has_ty lty2 sndc lty3 →
+      cmd_has_ty lty1 (SeqC fstc sndc) lty3
+  | LetTy: forall lty lhs e ty,
+      expr_has_ty lty e ty →
+      cmd_has_ty lty (LetC lhs e) (<[lhs := ty]>lty)
+  | IfTy: forall lty1 lty2 cond thn els,
+      expr_has_ty lty1 cond BoolT →
+      cmd_has_ty lty1 thn lty2 →
+      cmd_has_ty lty1 els lty2 →
+      cmd_has_ty lty1 (IfC cond thn els) lty2
+  | GetTy: forall lty lhs recv t name cdef fty,
+      expr_has_ty lty recv (ClassT t) →
+      Δ !! t = Some cdef →
+      cdef.(classfields) !! name = Some fty →
+      cmd_has_ty lty (GetC lhs recv name) (<[lhs := fty]>lty)
+  | SetTy: forall lty recv fld rhs fty t,
+      expr_has_ty lty recv (ClassT t) →
+      expr_has_ty lty rhs fty →
+      has_field fld fty t → (* TODO: subtyping ? *)
+      cmd_has_ty lty (SetC recv fld rhs) lty
+  | NewTy: forall lty lhs t args fields,
+      has_fields t fields →
+      dom (gset string) fields = dom _ args →
+      (forall f fty arg,
+        fields !! f = Some fty →
+        args !! f = Some arg →
+        expr_has_ty lty arg fty) →
+      cmd_has_ty lty (NewC lhs t args) (<[ lhs := ClassT t]>lty)
+  | CallTy: forall lty1 lty2 lhs recv t name args cdef mdef,
+      expr_has_ty lty1 recv (ClassT t) →
+      Δ !! t = Some cdef →
+      cdef.(classmethods) !! name = Some mdef →
+      dom (gset string) mdef.(methodargs) = dom _ args →
+      (forall x ty arg,
+      mdef.(methodargs) !! x = Some ty →
+      args !! x = Some arg →
+      expr_has_ty lty1 arg ty) →
+      cmd_has_ty lty1 mdef.(methodbody) lty2 →
+      expr_has_ty lty2 mdef.(methodret) mdef.(methodrettype) →
+      cmd_has_ty lty1 (CallC lhs recv name args) (<[ lhs := mdef.(methodrettype)]>lty1)
+.
+
+(* Big set reduction *)
+Definition primop_eval (op: primop) : Z -> Z -> value :=
+  match op with
+  | PlusO => fun x y => IntV (x + y)
+  | MinusO => fun x y => IntV (x - y)
+  | TimesO => fun x y => IntV (x * y)
+  | DivO => fun x y => IntV (x / y)
+  | LeqO => fun x y => BoolV (Z.leb x y)
+  | GeqO => fun x y => BoolV (Z.geb x y)
+  | EqO => fun x y => BoolV (Z.eqb x y)
+  end
+.
+
+Definition local_env := gmap var value.
+
+Fixpoint expr_eval (le : local_env) (e: expr) : option value :=
+  match e with
+  | IntE z => Some (IntV z)
+  | BoolE b => Some (BoolV b)
+  | NullE => Some NullV
+  | OpE op e1 e2 =>
+      match expr_eval le e1, expr_eval le e2 with 
+      | Some (IntV z1), Some (IntV z2) => Some (primop_eval op z1 z2)
+      | _, _ => None
+      end
+  | VarE v => le !! v
+  end
+.
 
 (* concrete heaps *)
 Definition heap : Type := gmap loc (tag * stringmap value).
+
+(*
+Definition map_args {A B: Type} (f: A → option  B) (m: stringmap A) : option (stringmap B) :=
+  let g (x: (string * A)) := f x.2 ≫= (fun y => mret (x.1, y)) in
+  mapM g (map_to_list m) ≫= (fun l => mret (list_to_map l))
+.
+
+Lemma dom_map_args: forall A B (f: A → option B)
+  (m: stringmap A) (n: stringmap B),
+  map_args f m = Some n -> 
+  dom stringset n = dom _ m.
+Proof.
+  move => A B f.
+  assert (h0: forall (l: list (string * A)) (k: list (string * B)),
+    mapM (λ x : string * A, f x.2 ≫= (λ y : B, mret (x.1, y))) l = Some k →
+    l.*1 = k.*1).
+  {
+    induction l as [ | [s0 ?] tl hi]; destruct k as [ | [s1 ?] tl'] => //.
+    - simpl.
+      destruct (f a) as [x | ] => //=.
+      by destruct mapM.
+    - simpl mapM.
+      destruct (f a) as [x | ] => //.
+      simpl mbind.
+      destruct mapM as [l | ] => //.
+      simpl mbind.
+      move => [= <- <- <-].
+      by rewrite !fmap_cons (hi l).
+  }
+  rewrite /map_args => m n h.
+  apply bind_Some in h as [l [hl h]].
+  apply h0 in hl.
+  injection h; intros <-; clear h.
+  rewrite dom_list_to_map_L -hl.
+  unfold_leibniz.
+  by rewrite dom_alt.
+Qed.
+
+
+Lemma map_args_lookup_: forall A B (f: A → option B) (l: list (string * A)) n,
+  NoDup l.*1 →
+  map_args f (list_to_map l) = Some n →
+  forall (m: stringmap A), m = list_to_map l →
+  forall k, n !! k = (m !! k) ≫= f.
+Proof.
+  move => A B f.
+  rewrite /map_args => l n hnodup h.
+  apply bind_Some in h as [l' [hl h]].
+  injection h; intros <-; clear h.
+  induction l as [ | [x v] tl hi]; destruct l' as [ | [y w] tl'] => //=.
+  - by move => m -> k.
+  - move => m -> k.
+    apply mapM_Some in hl.
+    apply Forall2_length in hl.
+    assert (hp: map_to_list (list_to_map ((x, v) :: tl)) ≡ₚ (x, v) :: tl) by (by apply map_to_list_to_map).
+    apply Permutation_length in hp.
+    by rewrite hl in hp.
+  - move => m -> k.
+    destruct (decide (y = k)) as [-> | hne0].
+    + rewrite lookup_insert.
+      destruct (decide (x = k)) as [-> | hne1].
+      * rewrite lookup_insert.
+        simpl in *.
+        apply mapM_Some in hl.
+
+  
+
+
+
+
+l : list (string * B)
+hl : mapM (λ x : string * A, f x.2 ≫= (λ y : B, mret (x.1, y)))
+       (map_to_list m) = Some l
+k : string
+
+========================= (1 / 1)
+
+list_to_map l !! k = m !! k ≫= f
+
+  Search mapM mbind.
+  apply mapM_Some in hl.
+  apply elem_of_mapM in hl.
+  Check elem_of_mapM.
+  Search mapM elem_of.
+  destruct (m !! k) as [ w | ] eqn:?.
+  Search elem_of lookup.
+  apply set_eq.
+  apply mapM_Some in hl.
+  apply Forall2_same_length_lookup in hl as [? hl].
+  Search list_to_map lookup.
+  destruct (map_to_list m !!
+  Search Forall2 lookup.
+  
+
+    Search list_to_map lookup.
+    Search map_to_list empty.
+    rewrite map_to_list_empty.
+    rewrite map_to_list_empty
+  Search map_to_list lookup.
+ *)
+
+Definition map_args {A B: Type} (f: A → option  B) (m: stringmap A) (n: stringmap B) :=
+  dom stringset m = dom stringset n /\
+  ∀ k a b, m !! k = Some a -> n !! k = Some b -> f a = Some b.
+
+Inductive cmd_eval:
+    (local_env * heap) → cmd →
+    (local_env * heap) → Prop :=
+  | SkipEv : forall st, cmd_eval st SkipC st
+  | LetEv: forall le h v e val,
+      expr_eval le e = Some val →
+      cmd_eval (le, h) (LetC v e) (<[v:=val]> le, h)
+  | NewEv: forall le h lhs new t args vargs,
+      h !! new = None →
+      (* map_args (expr_eval le) args = Some vargs → *)
+      map_args (expr_eval le) args vargs →
+      cmd_eval (le, h) (NewC lhs t args) (<[lhs := LocV new]>le, <[new := (t, vargs)]>h)
+  | GetEv: forall le h lhs recv name l t vs v,
+      expr_eval le recv = Some (LocV l) →
+      h !! l = Some (t, vs) →
+      vs !! name = Some v →
+      cmd_eval (le, h) (GetC lhs recv name) (<[lhs := v]>le, h)
+  | SetEv: forall le h recv fld rhs l v t vs vs',
+      expr_eval le recv = Some (LocV l) →
+      expr_eval le rhs = Some v →
+      h !! l = Some (t, vs) →
+      vs' = <[ fld := v ]>vs →
+      cmd_eval (le, h) (SetC recv fld rhs) (le, <[l := (t, vs')]> h)
+  | SeqEv: forall st1 st2 st3 fstc sndc,
+      cmd_eval st1 fstc st2 →
+      cmd_eval st2 sndc st3 →
+      cmd_eval st1 (SeqC fstc sndc) st3
+  | IfTrueEv: forall st1 st2 cond thn els,
+      expr_eval st1.1 cond = Some (BoolV true) →
+      cmd_eval st1 thn st2 →
+      cmd_eval st1 (IfC cond thn els) st2
+  | IfFalseEv: forall st1 st2 cond thn els,
+      expr_eval st1.1 cond = Some (BoolV false) →
+      cmd_eval st1 els st2 →
+      cmd_eval st1 (IfC cond thn els) st2
+  | CallEv: forall le h h' lhs recv l t vs name args vargs cdef mdef
+      run_env run_env' ret,
+      expr_eval le recv = Some (LocV l) →
+      (* map_args (expr_eval le) args = Some vargs → *)
+      map_args (expr_eval le) args vargs →
+      h !! l = Some (t, vs) →
+      Δ !! t = Some cdef →
+      cdef.(classmethods) !! name = Some mdef →
+      <["$this" := LocV l]>vargs = run_env →
+      cmd_eval (run_env, h) mdef.(methodbody) (run_env', h') →
+      expr_eval run_env' mdef.(methodret) = Some ret →
+      cmd_eval (le, h) (CallC lhs recv name args) (<[lhs := ret]>le, h')
+.
 
 (* heap models relation; the semantic heap does
    not appear because it is hidden in iProp  *)
 (* Helper defintion to state that fields are correctly modeled *)
 Definition heap_models_fields
-  (iFs: stringmap (laterO (sem_typeO Σ))) (vs: stringmap value) : iProp :=
+  (iFs: gmapO string (laterO (sem_typeO Σ))) (vs: stringmap value) : iProp :=
   ⌜dom (gset string) vs ≡ dom _ iFs⌝ ∗
   ∀ f (iF: interp),
   iFs !! f ≡ Some (Next iF) -∗ ∃ v, (⌜vs !! f = Some v⌝ ∗ ▷iF v).
 
+Lemma heap_models_fields_ext_L: forall iFs iFs' vs,
+  iFs ≡ iFs' -∗ heap_models_fields iFs vs -∗ heap_models_fields iFs' vs.
+Proof.
+  move => iFs iFs' vs.
+  iIntros "heq h".
+  rewrite /heap_models_fields.
+  iDestruct "h" as "[%hdom h]".
+  iSplit.
+  { rewrite gmap_equivI.
+    fold_leibniz.
+    rewrite set_eq hdom.
+    iIntros (s).
+    rewrite !elem_of_dom.
+    by iRewrite ("heq" $! s).
+  }
+  iIntros (f iF) "hiF".
+  iApply "h".
+  by iRewrite "heq".
+Qed.
+
 Definition heap_models (h : heap) : iProp :=
-  ∃ (sh: gmap loc (tag * stringmap (laterO (sem_typeO Σ)))),
+  ∃ (sh: gmap loc (prodO tagO (gmapO string (laterO (sem_typeO Σ))))),
     own γ (gmap_view_auth 1 sh) ∗ ⌜dom (gset loc) sh = dom _ h⌝ ∗
     □ ∀ (ℓ : loc) (t : tag) (vs : stringmap value),
       ⌜h !! ℓ = Some (t, vs)⌝ -∗
-        ∃ (iFs : stringmap (laterO (sem_typeO Σ))),
+        ∃ (iFs : gmapO string (laterO (sem_typeO Σ))),
         sh !! ℓ ≡ Some (t, iFs) ∗ heap_models_fields iFs vs.
-End proofs.
 
+Definition interp_local_tys
+    (lty : local_tys) (le : local_env) : iProp :=
+  (∀ v ty, ⌜lty !! v = Some ty⌝ -∗
+           ∃ val, ⌜le !! v = Some val⌝ ∗ interp_type ty val)%I.
+
+(*
+Lemma expr_typ_inv e le lty (h: heap) l t t0 vs:
+  (* missing link between le lty *)
+  expr_eval le e = Some (LocV l) →
+  h !! l = Some (t, vs) →
+  expr_has_ty lty e (ClassT t0) →
+  inherits t t0.
+Proof.
+  case: e => [z | b | | op e1 e2 | v] //=.
+  - destruct (expr_eval le e1) as [[z1| ? | | ?] | ] eqn:h1; move => //=.
+    destruct (expr_eval le e2) as [[z2| ? | | ?] | ] eqn:h2; move => //=.
+    move => [= hl] hh hexpr.
+    by inv hexpr.
+  - move => hle hh hexpr.
+    inv hexpr.
+ *)
+
+
+Lemma expr_adequacy e lty le ty val :
+  expr_eval le e = Some val →
+  expr_has_ty lty e ty →
+  interp_local_tys lty le -∗
+  interp_type ty val.
+Proof.
+  (* the language is this simple that no
+     induction is necessary *)
+  case: e => [z | b | | op e1 e2 | v] /=.
+  - move => [= <-] hexpr.
+    inv hexpr.
+    iIntros "_"; rewrite interp_type_unfold.
+    by iExists _.
+  - move => [= <-] hexpr.
+    inv hexpr.
+    iIntros "_"; rewrite interp_type_unfold.
+    by iExists _.
+  - move => [= <-] hexpr.
+    inv hexpr.
+    iIntros "_"; by rewrite interp_type_unfold.
+  - destruct (expr_eval le e1) as [[z1| ? | | ?] | ] eqn:h1; move => //=.
+    destruct (expr_eval le e2) as [[z2| ? | | ?] | ] eqn:h2; move => //=.
+    move => [= <-] hexpr.
+    inv hexpr.
+    + iIntros "hty".
+      rewrite interp_type_unfold /= /interp_int.
+      destruct op; by eauto.
+    + iIntros "hty".
+      rewrite interp_type_unfold /= /interp_bool.
+      destruct op; by eauto.
+  - move => hle hexpr.
+    inv hexpr.
+    iIntros "#Hlty".
+    iDestruct ("Hlty" with "[//]") as (?) "[% H]".
+    rewrite hle in H; injection H; intros <-; clear H.
+    done.
+Qed.
+
+Lemma interp_local_tys_update v lty le ty val :
+  interp_local_tys lty le -∗
+  interp_type ty val -∗
+  interp_local_tys (<[v:=ty]>lty) (<[v:=val]>le).
+Proof.
+  iIntros "#Hi #?". iIntros (v' ty') "H".
+  rewrite lookup_insert_Some.
+  iDestruct "H" as %[[<- <-]|[??]].
+  - iExists _. rewrite lookup_insert. by iSplit.
+  - rewrite lookup_insert_ne; last done. by iApply "Hi".
+Qed.
+
+Lemma heap_models_lookup l h A vs t :
+  h !! l = Some (t, vs) →
+  heap_models h -∗
+  interp_type (ClassT A) (LocV l) -∗
+  ∃ fields, heap_models h ∗
+    ⌜inherits t A ∧ has_fields t fields⌝ ∗
+    ∀ f fty, ⌜fields !! f = Some fty⌝ → 
+    ∃ v, ⌜vs !! f = Some v⌝ ∗
+    ▷ interp_type fty v.
+Proof.
+  move => hheap.
+  iIntros "hmodels hl".
+  rewrite interp_type_unfold /= /interp_class.
+  iDestruct "hl" as (???) "[%H H◯]".
+  destruct H as [[= <-] [hinherits hf]].
+  iDestruct "hmodels" as (sh) "(H● & % & #Hh)".
+  iDestruct (own_valid_2 with "H● H◯") as "#Hv".
+  rewrite gmap_view_both_validI.
+  iDestruct "Hv" as "[_ HΦ]".
+  iDestruct ("Hh" with "[//]") as (?) "[H H▷]".
+  iRewrite "H" in "HΦ".
+  rewrite option_equivI prod_equivI /=.
+  iDestruct "HΦ" as "[-> HΦ]".
+  iExists fields.
+  iSplitL. { iExists _. iFrame. by iSplit. }
+  iSplitR; first by rewrite H0.
+  iIntros (f fty) "%hfield".
+  iDestruct "H▷" as "[%hdf h]".
+  rewrite gmap_equivI.
+  iSpecialize ("HΦ" $! f).
+  rewrite /interp_tys_next /interp_ty_next lookup_fmap hfield /=.
+  iAssert (⌜is_Some (iFs !! f)⌝)%I as "%hiFs".
+  { destruct (iFs !! f) eqn:hh; first done.
+    by rewrite hh option_equivI.
+  }
+  destruct hiFs as [[iF] hIF].
+  iDestruct ("h" $! f iF with "[]") as (v) "[%hv hl]"; first by rewrite hIF.
+  iExists v; iSplitR; first done.
+  rewrite hIF option_equivI later_equivI discrete_fun_equivI.
+  iNext.
+  iSpecialize ("HΦ" $! v).
+  by iRewrite -"HΦ".
+Qed.
+
+Lemma heap_models_fields_update iFs vs f v (Φ : interpO)
+  `{∀ v, Persistent (Φ v)} :
+  iFs !! f = Some (Next Φ) ->
+  heap_models_fields iFs vs -∗
+  Φ v -∗
+  heap_models_fields iFs (<[ f := v]>vs).
+Proof.
+  move => hf.
+  iIntros "hm hΦ".
+  iDestruct "hm" as "[%hdom h]".
+  rewrite /heap_models_fields.
+  iSplitR.
+  { iPureIntro.
+    rewrite dom_insert_lookup //.
+    by rewrite -elem_of_dom hdom elem_of_dom hf.
+  }
+  iIntros (f' iF) "hf".
+  destruct (decide (f = f')) as [-> | hne].
+  - rewrite lookup_insert.
+    iExists v; iSplitR; first done.
+    rewrite hf option_equivI later_equivI discrete_fun_equivI.
+    iNext.
+    iSpecialize ("hf" $! v).
+    by iRewrite -"hf".
+  - rewrite lookup_insert_ne //.
+    by iApply "h".
+Qed.
+
+Lemma heap_models_update h l t t0 vs f v fty:
+  wf_cdefs Δ ->
+  h !! l = Some (t, vs) ->
+  has_field f fty t0 ->
+  inherits t t0 ->
+  heap_models h -∗
+  interp_type (ClassT t0) (LocV l) -∗
+  interp_type fty v -∗
+  heap_models (<[l:=(t, (<[f := v]>vs))]> h).
+Proof.
+  move => wfΔ hheap hf hinherits.
+  iIntros "hmodels #hl #hv".
+  iDestruct "hmodels" as (sh) "[hown [%hdom #h]]".
+  iExists sh.
+  rewrite interp_type_unfold /= /interp_class.
+  iDestruct "hl" as (?? fields) "[%H hsem]".
+  destruct H as [[= <-] [ hinherits' hfields]].
+  iDestruct (own_valid_2 with "hown hsem") as "#Hv".
+  rewrite gmap_view_both_validI.
+  iDestruct "Hv" as "[_ Hv]".
+  iSplitL; first by iFrame.
+  iSplitR.
+  { iPureIntro.
+    by rewrite hdom dom_insert_lookup_L.
+  }
+  iModIntro.
+  iIntros (ℓ t' vs') "%Heq".
+  destruct (decide (l = ℓ)) as [-> | hne].
+  - rewrite lookup_insert in Heq.
+    injection Heq; intros <- <-; clear Heq.
+    iAssert (t1 ≡ t)%I as "%Ht".
+    { iSpecialize ("h" $! ℓ t vs with "[//]").
+      iDestruct "h" as (iFs) "[hsh hmodels]".
+      iRewrite "Hv" in "hsh".
+      rewrite !option_equivI prod_equivI /=.
+      by iDestruct "hsh" as "[? ?]".
+    }
+    iExists _; iSplitR.
+    { rewrite Ht.
+      by iRewrite "Hv".
+    }
+    iApply heap_models_fields_update; first by apply interp_type_persistent.
+    + rewrite /interp_tys_next /interp_ty_next lookup_fmap.
+      destruct (hfields f fty) as [h0 h1].
+      rewrite h0; first by done.
+      by apply has_fields_inherits with t0.
+    + iSpecialize ("h" $! ℓ t vs with "[//]").
+      iDestruct "h" as (iFs) "[hsh hmodels]".
+      iRewrite "Hv" in "hsh".
+      rewrite !option_equivI prod_equivI /=.
+      iDestruct "hsh" as "[? h]".
+      iApply heap_models_fields_ext_L; first by iRewrite "h".
+      done.
+    + done.
+  - iApply "h".
+    iPureIntro.
+    by rewrite lookup_insert_ne // in Heq.
+Qed.
+
+Notation "|=▷^ n Q" := (Nat.iter n (λ P, |==> ▷ P) Q)%I
+  (at level 99, n at level 9, Q at level 200,
+   format "|=▷^ n  Q") : bi_scope.
+
+Lemma updN_zero (Q : iProp) : (|=▷^0 Q) ⊣⊢ Q.
+Proof. done. Qed.
+
+Lemma updN_S n (Q : iProp) :
+  (|=▷^(S n) Q) ⊣⊢ |==> ▷ |=▷^n Q.
+Proof. done. Qed.
+
+Lemma updN_mono n (P Q : iProp) :
+  (P -∗ Q) → (|=▷^n P) -∗ (|=▷^n Q).
+Proof.
+  elim: n => [//|n HI H].
+  rewrite !updN_S.
+  iApply bupd_mono.
+  iApply bi.later_mono.
+  by iApply HI.
+Qed.
+
+Lemma cmd_adequacy lty lty' st cmd st' :
+  wf_cdefs Δ →
+  cmd_eval st cmd st' →
+  cmd_has_ty lty cmd lty' →
+  ∃ n,
+    heap_models st.2 ∗ interp_local_tys lty st.1 -∗ |=▷^n
+    heap_models st'.2 ∗ interp_local_tys lty' st'.1.
+Proof.
+  move=> wfΔ E. move: lty lty'. elim: E.
+  - move => ? lty lty' hty.
+    inv hty.
+    by exists 0.
+  - move=> le h lhs recv val hrecv /=.
+    exists 0. iIntros "[? #Hle]".
+    rewrite updN_zero. iFrame.
+    inv H.
+    iDestruct (expr_adequacy with "Hle") as "#?"; try done.
+    by iApply interp_local_tys_update.
+  - move => le h lhs new t args vargs hnew hargs lty lty' hc /=.
+    inv hc.
+    exists 1. iIntros "[Hh #Hle]".
+    (* we need one modality to update the
+       semantic heap *)
+    rewrite updN_S updN_zero.
+    iDestruct "Hh" as (sh) "(H●&Hdom&#Hh)".
+    iDestruct "Hdom" as %Hdom.
+    iMod (own_update with "H●") as "[H● H◯]".
+    { apply (gmap_view_alloc _ new DfracDiscarded
+        (t, interp_tys_next interp_type fields)); last done.
+      apply (not_elem_of_dom (D:=gset loc)).
+      by rewrite Hdom not_elem_of_dom. }
+    iIntros "!> !>". iDestruct "H◯" as "#H◯".
+    iAssert (interp_type (ClassT t) (LocV new))
+      with "[]" as "#Hl".
+    { rewrite interp_type_unfold /=.
+      iExists _, _, _. by iSplit. }
+    iSplitL; last first.
+    by iApply interp_local_tys_update.
+    iExists _. iFrame. iSplit.
+    by rewrite !dom_insert_L Hdom.
+    iModIntro. iIntros (???) "Hlook".
+    rewrite lookup_insert_Some.
+    iDestruct "Hlook" as %[[<- [= <- <-]]|[Hℓ Hlook]].
+    + iExists _. rewrite lookup_insert.
+      iSplitR; first done.
+      rewrite /heap_models_fields.
+      destruct hargs as [hargsdom hargs]. 
+      iSplitR.
+      { 
+        by rewrite dom_interp_tys_next -hargsdom H5.
+      }
+      iIntros (f iF) "hiF".
+      iAssert (⌜f ∈ dom stringset fields⌝)%I as "%hf".
+      {
+        rewrite -dom_interp_tys_next elem_of_dom.
+        rewrite /interp_tys_next /interp_ty_next.
+        rewrite !lookup_fmap.
+        by iRewrite "hiF".
+      }
+      assert (h0: is_Some (args !! f)).
+      {
+        apply elem_of_dom.
+        by rewrite -H5.
+      }
+      destruct h0 as [a0 ha0].
+      assert (h1: is_Some (vargs !! f)).
+      {
+        apply elem_of_dom.
+        by rewrite -hargsdom -H5.
+      }
+      destruct h1 as [v0 hv0].
+      assert (h2: is_Some (fields !! f)) by (by apply elem_of_dom).
+      destruct h2 as [fty hty].
+      iExists v0; iSplitR; first done.
+      rewrite /interp_tys_next /interp_ty_next lookup_fmap.
+      assert (heval0: expr_eval le a0 = Some v0) by (by apply hargs with f).
+      assert (hty0: expr_has_ty lty a0 fty) by (by apply H6 with f).
+      rewrite hty /= option_equivI later_equivI.
+      iNext.
+      rewrite discrete_fun_equivI.
+      iSpecialize ("hiF" $! v0).
+      iRewrite -"hiF".
+      by iDestruct (expr_adequacy a0 with "Hle") as "#Ha0".
+    + rewrite lookup_insert_ne; last done.
+      by iApply "Hh".
+  - move => le h hls recv name l t vs v hle hh hvs lty lty' hc.
+    inv hc.
+    exists 1. iIntros "[Hh #Hle]". simpl.
+    iModIntro. (* keep the later *)
+    iDestruct (expr_adequacy with "Hle") as "#He"; try done.
+    iDestruct (heap_models_lookup with "Hh He") as (fields) "(Hh&Ht&Hv)"; first done.
+    iDestruct "Ht" as %[? ?].
+    rewrite bi.later_sep.
+    iSplitL "Hh"; first done.
+    assert (hf: fields !! name = Some fty) by (by apply (has_fields_inherits_lookup wfΔ) with t t0 cdef).
+    iDestruct ("Hv" $! name fty hf) as (w) "[%hw hi]".
+    rewrite hvs in hw; injection hw; intros ->; clear hw.
+    iNext. by iApply interp_local_tys_update.
+  - move => le h recv fld rhs l v t vs vs' hrecv hrhs hh -> lty lty' hcmd.
+    inv hcmd.
+    exists 0.
+    iIntros "[Hh #Hle]".
+    rewrite updN_zero /=. iSplitL; last done.
+    iDestruct (expr_adequacy recv with "Hle") as "#Hrecv" => //.
+    iDestruct (expr_adequacy rhs with "Hle") as "#Hrhs" => //.
+    iDestruct (heap_models_lookup with "Hh Hrecv") as (fields) "(Hh&Ht&?)"; first done.
+    iDestruct "Ht" as %[? ?].
+    by iApply (heap_models_update with "Hh").
+  - move => st1 st2 st3 fstc sndc hcfst hfst hcsnd hsnd lty lty' h.
+    inv h.
+    apply hfst in H2. apply hsnd in H4.
+    clear hfst hsnd.
+    destruct H2 as [n1 Hfst].
+    destruct H4 as [n2 Hsnd].
+    exists (n1 + n2).
+    iIntros "H".
+    iDestruct (Hfst with "H") as "H".
+    iPoseProof (updN_mono with "H") as "H";
+      first done.
+    by rewrite Nat_iter_add.
+  - move => st1 st2 cond thn els hexpr hcthn hi hcels hels h.
+    inv h.
+    apply hi in H5. clear hi.
+    destruct H5 as [n Hifc]. exists n.
+    iIntros "H". iPoseProof (Hifc with "H") as "H".
+    done.
+  - move => st1 st2 cond thn els hexpr hcthn hi hcels hels h.
+    inv h.
+    apply hi in H6. clear hi.
+    destruct H6 as [n Helc]. exists n.
+    iIntros "H". iPoseProof (Helc with "H") as "H".
+    done.
+  - move => le h h' lhs recv l t vs name args vargs cdef mdef run_env
+    run_env' ret hrecv hargs hh hΔ hcdef <- hbody hi hret lty lty' hc.
+    inv hc.
+    (* t should inherits t0 *)
+    (* WIP *)
+    (* Need stuff about methods like we did properties (override, ...) *)
+    admit.
+Admitted.
+    
 (* Thank you Robbert. TODO: update iris to get it from it *)
 Global Instance gmap_dom_ne n `{Countable K} {A : ofe}:
   Proper ((≡{n}@{gmap K A}≡) ==> (=)) (dom (gset K)).
 Proof. intros m1 m2 Hm. apply set_eq=> k. by rewrite !elem_of_dom Hm. Qed.
-
-Section Examples.
-Context `{!sem_heapG Σ}.
-Notation iProp := (iProp Σ).
-Context (γ : gname).
-Notation interpO := (sem_typeO Σ).
-
-Definition sem_heap_mapsto ℓ t (iFs: gmapO string (laterO interpO)) :=
-  (own γ (gmap_view_frag ℓ DfracDiscarded (t, iFs))).
-
-(*
-class C {
-  int $foo;
-}
-
-class D extends C {
-  D $rec;
-}
-*)
-Definition C : classDef := {|
-  classname := "C";
-  classmethods := ∅;
-  superclass := None;
-  classfields := {["foo" := IntT]};
-  |}.
-
-Definition D : classDef := {|
-  classname := "D";
-  classmethods := ∅;
-  superclass := Some "C";
-  classfields := {["rec" := ClassT "D"]};
-  |}.
-
-Definition Δ: stringmap classDef :=
-  <["D" := D]>{["C" := C]}.
-
-Fact C_field : forall fname ty,
-  has_field Δ fname ty "C" <-> (fname = "foo" /\ ty = IntT).
-Proof.
-move => fname typ; split => [hf | [-> ->]].
-- inversion hf; subst; clear hf.
-  + rewrite /Δ /= lookup_insert_ne //= lookup_insert in H.
-    injection H; intros <-; clear H.
-    destruct (string_eq_dec fname "foo") as [he | hne] eqn:?.
-    { subst; split; first done.
-      rewrite /C lookup_insert /= in H0.
-      by injection H0.
-    }
-    by rewrite /C lookup_insert_ne //= in H0.
-  + rewrite /Δ /= lookup_insert_ne //= lookup_insert in H.
-    injection H; intros <-; clear H.
-    by elim H1.
-- econstructor; first by done.
-  by rewrite /C lookup_insert //=.
-Qed.
-
-Fact D_field : forall fname typ,
-  has_field Δ fname typ "D" <->
-  ((fname = "foo" /\ typ = IntT) \/ (fname = "rec" /\ typ = ClassT "D")).
-Proof.
-move => f; split => [hf | [ [-> ->] | [-> ->]]].
-- inversion hf; subst; clear hf.
-  + rewrite /Δ //= lookup_insert in H.
-    injection H; intros <-; clear H.
-    destruct (string_eq_dec f "foo") as [-> | hne]; first by subst.
-    destruct (string_eq_dec f "rec") as [-> | hne2].
-    { right; split; first done.
-      rewrite /D lookup_insert /= in H0.
-      by injection H0.
-    }
-    by rewrite /C lookup_insert_ne //= in H0.
-  + rewrite /Δ //= lookup_insert in H.
-    injection H; intros <-; clear H.
-    rewrite /D /= in H1.
-    injection H1; intros <-; clear H1.
-    apply C_field in H2; now subst; left.
-- eapply InheritsField; [ done | done | done | by apply C_field].
-- econstructor; first by done.
-  by rewrite /C lookup_insert //=.
-Qed.
-
-(* Sanity checks for fields and inheritance *)
-Lemma check_fields_C : has_fields Δ "C" {["foo" := IntT]}.
-Proof.
-move => f; split => [h | h].
-- by apply C_field in h as [-> ->].
-- by econstructor.
-Qed.
-
-Lemma check_fields_D :
-  has_fields Δ "D" ({["foo" := IntT; "rec" := ClassT "D"]}).
-Proof.
-move => f; split => [h | ].
-- inversion h; subst; clear h.
-  + destruct (string_eq_dec f "rec") as [-> | hnrec] eqn:hdrec.
-    { rewrite lookup_insert_ne //= lookup_insert.
-      rewrite /Δ  lookup_insert in H.
-      injection H; intros <-; clear H.
-      by rewrite /D lookup_insert in H0.
-    }
-    rewrite /Δ lookup_insert in H.
-    injection H; intros <-; clear H.
-    by rewrite lookup_insert_ne //= in H0.
-  + rewrite /Δ lookup_insert in H.
-    injection H; intros <-; clear H.
-    rewrite /D /= in H1.
-    injection H1; intros <-; clear H1.
-    by apply C_field in H2 as [-> ->].
-- rewrite lookup_insert_Some => h.
-  destruct h as [ [<- <-] | [hne h]].
-  { apply D_field; by left. }
-  by econstructor.
-Qed.
-
-Example alloc_unit_class_lemma (h : heap) (new : loc) :
-  h !! new = None →
-  heap_models γ h -∗ |==>
-   heap_models γ (<[ new := ("C", {[ "foo" := IntV 0 ]}) ]> h) ∗
-   sem_heap_mapsto new "C" {[ "foo" := Next (interp_type Δ γ IntT)]}.
-Proof.
-  move=> Hnew. iIntros "Hm". iDestruct "Hm" as (sh) "[Hown [Hdom #Hm]]".
-  iDestruct "Hdom" as %Hdom.
-  iMod (own_update with "Hown") as "[Hown Hfrag]".
-  { apply (gmap_view_alloc _ new DfracDiscarded); last done.
-    (* the typeclasses seem to be messed up below, I should be able
-       to use not_elem_of_dom directly *)
-    move: Hnew. rewrite -!(@not_elem_of_dom _ _ (gset loc)).
-    by move: Hdom => ->. }
-  iIntros "!>". iFrame.
-  iExists _. iFrame. iSplitR.
-  { iPureIntro. rewrite !dom_insert_L.
-    by move: Hdom => ->. }
-  iModIntro.
-  iIntros (ℓ t vs) "Hlook".
-  rewrite lookup_insert_Some.
-  iDestruct "Hlook" as %[[<- [= <- <-]]|[Hℓ Hlook]].
-  - iExists _. rewrite lookup_insert.
-    iSplitR; first done.
-    rewrite /heap_models_fields.
-    iSplitR.
-    { iPureIntro. by rewrite !dom_insert_L !dom_empty_L. }
-    iIntros (f iF).
-    destruct (string_eq_dec f "foo") as [-> | hne]; last first.
-    { rewrite !lookup_insert_ne //= !lookup_empty option_equivI.
-      by iIntros "hfalse".
-    }
-    rewrite !lookup_insert option_equivI later_equivI.
-    iIntros "Hf".
-    iExists (IntV 0); iSplit; first done.
-    iNext.
-    rewrite discrete_fun_equivI /=.
-    iSpecialize ("Hf" $! (IntV 0)).
-    iRewrite -"Hf".
-    rewrite interp_type_unfold /= /interp_int.
-    by iExists 0.
-  - iDestruct ("Hm" with "[]") as (iFs) "[Hin [hidom hisem]]"; first done.
-    rewrite /heap_models_fields.
-    iExists _. rewrite lookup_insert_ne; last done.
-    iSplitR; first by done.
-    by iSplitR.
-Qed.
-
-Remark inheritsD: forall t, ancestor Δ "D" t -> t = "D".
-Proof.
-move => t h.
-inversion h; subst; clear h; first done.
-destruct cdef as [classname superclass ? ?]; simpl in *.
-destruct (string_eq_dec t "D") as [-> | hne]; first done.
-destruct (string_eq_dec t "C") as [-> | hne2].
-- rewrite lookup_insert_ne in H; last by done.
-  simpl in *.
-  rewrite lookup_insert /= in H.
-  by injection H; intros; subst; clear H.
-- by rewrite !lookup_insert_ne //= in H.
-Qed.
-
-Example alloc_unit_class_lemma_rec (h : heap) (l : loc) frag:
-  h !! l = Some ("D", frag) →
-  interp_type Δ γ (ClassT "D") (LocV l) -∗
-  heap_models γ h -∗
-  heap_models γ (<[ l := ("D", <["rec" := LocV l]>frag) ]> h).
-Proof.
-  move => hbefore.
-  iIntros "#Hsem Hm".
-  iDestruct "Hm" as (sh) "[H● [%Hdom #Hm]]".
-  rewrite interp_type_unfold /= /interp_class.
-  iDestruct "Hsem" as (???) "[%hh #H◯]".
-  destruct hh as [[= <-] [hext hfields]].
-  apply inheritsD in hext; subst.
-  eapply has_fields_fun in hfields; last by apply check_fields_D.
-  destruct (sh !! l)  as [ [t iFs] | ] eqn:Hsh; last first.
-  {
-    assert (hl : l ∈ dom (gset loc) h); first by apply elem_of_dom.
-    assert (hl': l ∉ dom (gset loc) sh); first by apply not_elem_of_dom.
-    rewrite Hdom in hl'.
-    now elim hl'.
-  }
-  iDestruct (own_valid_2 with "H● H◯") as "#Hv".
-  rewrite gmap_view_both_validI.
-  iDestruct "Hv" as "[_ Hsh]".
-  rewrite Hsh option_equivI prod_equivI /interp_tys_next /interp_ty_next /=.
-  iDestruct "Hsh" as "#[%Heqt Heqi]".
-  (* Hm needs to be persistent (hence the □) otherwise
-     we would kill it here to get interp_type for l's
-     field but we would also need it later to show
-     heap_models *)
-  iDestruct ("Hm" $! l "D" frag with "[//]") as (?) "[Hsh [%Hdom2 Hvs]]".
-  rewrite Hsh option_equivI prod_equivI /=.
-  iDestruct "Hsh" as "[%Hl Hr]".
-  fold_leibniz.
-  rewrite Hl in Hsh.
-  clear t Heqt Hl.
-  (* we now show heap_models of the new heap *)
-  iExists sh. iFrame.
-  have -> : dom (gset loc) (<[l:=("D", <["rec":=LocV l]>frag)]>h) = dom _ h.
-  { by apply dom_insert_lookup_L. }
-  iSplitL; first done.
-  iModIntro. iIntros (???) "Hlook".
-  rewrite lookup_insert_Some.
-  iDestruct "Hlook" as %[[<- [= <- <-]]|[Hℓ Hlook]]; last by iApply "Hm".
-  iExists iFs. 
-  iSplitL; first by rewrite Hsh.
-  rewrite /heap_models_fields.
-  iSplit.
-  {
-    rewrite dom_insert Hdom2.
-    iRewrite -"Hr".
-    iRewrite "Heqi".
-    iPureIntro.
-    by set_solver.
-  }
-  iIntros (f iF) "hIF".
-  destruct (string_eq_dec f "rec") as [-> | hf]; last first.
-  - rewrite lookup_insert_ne //=.
-    iApply "Hvs".
-    iRewrite -"hIF".
-    by iRewrite "Hr".
-  - rewrite lookup_insert.
-    iExists (LocV l); iSplitR; first done.
-    rewrite gmap_equivI.
-    iSpecialize ("Heqi" $! "rec").
-    rewrite lookup_fmap.
-    rewrite -hfields lookup_insert_ne //= lookup_insert /=.
-    iRewrite "Heqi" in "hIF".
-    rewrite !option_equivI later_equivI.
-    iNext.
-    rewrite discrete_fun_equivI.
-    iSpecialize ("hIF" $! (LocV l)).
-    iRewrite -"hIF".
-    rewrite interp_type_unfold /= /interp_class /=.
-    iExists _, _, _.
-    iSplitR; last done.
-    { iPureIntro.
-      split; first done.
-      split; first by constructor.
-      by apply check_fields_D.
-    }
-Qed.
-
-Definition one_shot_loop_sh : stringmap (laterO (sem_typeO Σ)) :=
-  {[
-    "foo" := Next (interp_type Δ γ IntT);
-    "rec" := Next (interp_type Δ γ (ClassT "D"))
-    ]}.
-
-Example one_shot_loop (h : heap) (new : loc):
-  h !! new = None →
-  heap_models γ h -∗ |==>
-      heap_models γ (<[ new := ("D", {[ "foo" := IntV 0; "rec" := LocV new]}) ]> h) ∗
-      sem_heap_mapsto new "D" one_shot_loop_sh.
-Proof.
-  move=> Hl. iIntros "Hh".
-  iDestruct "Hh" as (sh) "[H● [%Hdom #Hm]]".
-  iMod (own_update with "H●") as "[H● H◯]".
-  { apply (gmap_view_alloc _ new DfracDiscarded); last done.
-    apply (not_elem_of_dom (D:=gset loc)).
-    by rewrite Hdom not_elem_of_dom. }
-  iDestruct "H◯" as "#H◯".
-  iModIntro.
-  iSplit; last done.
-  iExists _. iFrame. iSplitR.
-  { iPureIntro. rewrite !dom_insert_L.
-    by rewrite Hdom. }
-  iModIntro. iIntros (l' t' v) "H".
-  rewrite lookup_insert_Some.
-  iDestruct "H" as %[[<- [= <- <-]]|[??]].
-  - iExists one_shot_loop_sh. rewrite lookup_insert.
-    rewrite option_equivI /=.
-    iSplitR; first done.
-    rewrite /heap_models_fields.
-    iSplitR; first by iPureIntro.
-    iIntros (f iF) "hos".
-    rewrite /one_shot_loop_sh.
-    destruct (string_eq_dec f "foo") as [-> | hne0].
-    { rewrite !lookup_insert /= option_equivI later_equivI.
-      iExists (IntV 0); iSplitR; first by iPureIntro.
-      iNext.
-      rewrite discrete_fun_equivI.
-      iSpecialize ("hos" $! (IntV 0)).
-      iRewrite -"hos".
-      rewrite interp_type_unfold /= /interp_int.
-      now iExists 0.
-    }
-    destruct (string_eq_dec f "rec") as [-> | hne1].
-    { rewrite lookup_insert_ne // lookup_insert.
-      rewrite lookup_insert_ne // lookup_insert option_equivI later_equivI.
-      iExists (LocV new); iSplitR; first by iPureIntro.
-      iNext.
-      rewrite discrete_fun_equivI.
-      iSpecialize ("hos" $! (LocV new)).
-      iRewrite -"hos".
-      rewrite interp_type_unfold /= /interp_class.
-      iExists new, "D", ({["foo" := IntT; "rec" := ClassT "D"]}).
-      iSplitR.
-      { iPureIntro; split; first done.
-        split; first constructor.
-        by apply check_fields_D.
-      }
-      rewrite /interp_tys_next /interp_ty_next /=.
-      rewrite !fmap_insert fmap_empty.
-      done.
-    }
-    rewrite !lookup_insert_ne //= lookup_empty.
-    rewrite option_equivI.
-    done.
-  - iDestruct ("Hm" $! l' with "[//]") as (iF) "[??]".
-    iExists _. rewrite lookup_insert_ne; last done.
-    iSplit; eauto.
-Qed.
-
-End Examples.
